Makefile
@@ -1,7 +1,8 @@
 COQFLAGS := `cat _CoqProject`
 COQC := coqc $(COQFLAGS)
 
-VFILES := RunLength Instances NatEncode Ord MergesortClass Prefix BurrowsWheeler
+VFILES := RunLength Instances NatEncode Ord Mergesort Prefix BurrowsWheeler Sorted \
+					Rotation Iterate
 
 all: $(addsuffix .vo, $(VFILES))
 
@@ -14,15 +15,16 @@ clean:
 RunLength.vo: Instances.vo NatEncode.vo SumboolIf.vo \
 							VST/compcert/lib/Integers.vo \
 							VST/compcert/lib/Coqlib.vo
-Instances.vo: VST/msl/eq_dec.vo VST/compcert/lib/Integers.vo
+Instances.vo: VST/msl/eq_dec.vo VST/compcert/lib/Integers.vo Ord.vo
 NatEncode.vo: VST/compcert/lib/Integers.vo
-Ord.vo: VST/compcert/lib/Integers.vo Instances.vo
-MergesortClass.vo: Ord.vo
-Prefix.vo: Ord.vo MergesortClass.vo
+Ord.vo: VST/compcert/lib/Integers.vo
+Mergesort.vo: Ord.vo Sorted.vo
+Prefix.vo: Ord.vo Mergesort.vo
 BurrowsWheeler.vo: Ord.vo Rotation.vo Prefix.vo Rots.vo
 Rotation.vo: Repeat.vo
 Iterate.vo: Repeat.vo
 Rots.vo: Iterate.vo Rotation.vo Repeat.vo
+Sorted.vo: Ord.vo
 
 VST/%.vo: VST/%.v
 	$(MAKE) -C VST $(patsubst VST/%,%,$@)
